src/opt/Simulation.v
@@ -40,27 +40,29 @@ Section Simulation.
       (MEM_FUTURE_TGT: Memory.future mem0_tgt mem1_tgt),
       <<TERMINAL:
         forall (TERMINAL_TGT: Threads.is_terminal ths1_tgt),
-        exists ths2_src sc2_src mem2_src,
-          <<STEPS_SRC: rtc Configuration.tau_step (Configuration.mk ths1_src sc1_src mem1_src) (Configuration.mk ths2_src sc2_src mem2_src)>> /\
-          <<SC: TimeMap.le sc2_src sc1_tgt>> /\
-          <<MEMORY: sim_memory mem2_src mem1_tgt>> /\
-          <<TERMINAL_SRC: Threads.is_terminal ths2_src>>>> /\
+          <<ABORT: Configuration.steps_abort (Configuration.mk ths1_src sc1_src mem1_src)>> \/
+          exists ths2_src sc2_src mem2_src,
+            <<STEPS_SRC: rtc Configuration.tau_step (Configuration.mk ths1_src sc1_src mem1_src) (Configuration.mk ths2_src sc2_src mem2_src)>> /\
+            <<SC: TimeMap.le sc2_src sc1_tgt>> /\
+            <<MEMORY: sim_memory mem2_src mem1_tgt>> /\
+            <<TERMINAL_SRC: Threads.is_terminal ths2_src>>>> /\
       <<STEP:
         forall e tid_tgt ths3_tgt sc3_tgt mem3_tgt
           (STEP_TGT: Configuration.step e tid_tgt (Configuration.mk ths1_tgt sc1_tgt mem1_tgt) (Configuration.mk ths3_tgt sc3_tgt mem3_tgt)),
-        exists tid_src ths2_src sc2_src mem2_src ths3_src sc3_src mem3_src,
-          <<STEPS_SRC: rtc Configuration.tau_step (Configuration.mk ths1_src sc1_src mem1_src) (Configuration.mk ths2_src sc2_src mem2_src)>> /\
-          <<STEP_SRC: Configuration.opt_step e tid_src (Configuration.mk ths2_src sc2_src mem2_src) (Configuration.mk ths3_src sc3_src mem3_src)>> /\
-          <<SC3: TimeMap.le sc3_src sc3_tgt>> /\
-          <<MEMORY3: sim_memory mem3_src mem3_tgt>> /\
-          <<SIM: sim ths3_src sc3_src mem3_src ths3_tgt sc3_tgt mem3_tgt>>>>.
+          <<ABORT: Configuration.steps_abort (Configuration.mk ths1_src sc1_src mem1_src)>> \/
+          exists tid_src ths2_src sc2_src mem2_src ths3_src sc3_src mem3_src,
+            <<STEPS_SRC: rtc Configuration.tau_step (Configuration.mk ths1_src sc1_src mem1_src) (Configuration.mk ths2_src sc2_src mem2_src)>> /\
+            <<STEP_SRC: Configuration.opt_step e tid_src (Configuration.mk ths2_src sc2_src mem2_src) (Configuration.mk ths3_src sc3_src mem3_src)>> /\
+            <<SC3: TimeMap.le sc3_src sc3_tgt>> /\
+            <<MEMORY3: sim_memory mem3_src mem3_tgt>> /\
+            <<SIM: sim ths3_src sc3_src mem3_src ths3_tgt sc3_tgt mem3_tgt>>>>.
 
   Lemma _sim_mon: monotone6 _sim.
   Proof.
     ii. exploit IN; try apply SC1; eauto. i. des.
     splits; eauto. i.
-    exploit STEP; eauto. i. des.
-    esplits; eauto.
+    exploit STEP; eauto. i. des; eauto.
+    right. esplits; eauto.
   Qed.
   Hint Resolve _sim_mon: paco.
 
